Some attempt in backward call rule.

floyd/SeparationLogicFacts.v
@@ -11,6 +11,133 @@ Export SeparationLogicSoundness.SoundSeparationLogic.CSL.
 Require Import VST.veric.NullExtension.
 Local Open Scope logic.
 
+(* Closed and subst. copied from closed_lemmas.v. *)
+
+Lemma closed_wrt_subst:
+  forall {A} id e (P: environ -> A), closed_wrt_vars (eq id) P -> subst id e P = P.
+Proof.
+intros.
+unfold subst, closed_wrt_vars in *.
+extensionality rho.
+symmetry.
+apply H.
+intros.
+destruct (eq_dec id i); auto.
+right.
+rewrite Map.gso; auto.
+Qed.
+
+(* End of copied from closed_lemmas.v. *)
+
+Definition obox (i: ident) (P: environ -> mpred): environ -> mpred :=
+  (fun rho => P (mkEnviron (ge_of rho) (ve_of rho) (Map.remove i (te_of rho)))) &&  ALL v: _, subst i (`v) P.
+
+Definition odia (i: ident) (P: environ -> mpred): environ -> mpred :=
+  (fun rho => P (mkEnviron (ge_of rho) (ve_of rho) (Map.remove i (te_of rho)))) || EX v: _, subst i (`v) P.
+
+Lemma subst_obox: forall id v (P: environ -> mpred), subst id (`v) (obox id P) = obox id P.
+Proof.
+  intros.
+  apply closed_wrt_subst.
+  hnf; intros.
+  unfold obox; simpl.
+  f_equal.
+  + f_equal.
+    f_equal.
+    apply Map.ext; intros j.
+    destruct (ident_eq id j).
+    - subst.
+      rewrite !Map.grs; auto.
+    - rewrite !Map.gro by congruence.
+      destruct (H j); [congruence |].
+      auto.
+  + apply allp_congr; intros.
+    unfold subst.
+    simpl.
+    f_equal.
+    unfold_lift.
+    unfold env_set.
+    f_equal.
+    simpl.
+    apply Map.ext; intros j.
+    destruct (ident_eq id j).
+    - subst.
+      rewrite !Map.gss; auto.
+    - rewrite !Map.gso by congruence.
+      destruct (H j); [congruence |].
+      auto.
+Qed.
+
+Lemma obox_T: forall i (P: environ -> mpred),
+  obox i P |-- P.
+Proof.
+  intros.
+  intro rho; simpl.
+  destruct (Map.get (te_of rho) i) eqn:?H.
+  + unfold obox; simpl.
+    apply andp_left2.
+    apply (allp_left _ v).
+    unfold subst.
+    apply derives_refl'.
+    f_equal.
+    unfold_lift.
+    destruct rho.
+    unfold env_set; simpl in *.
+    f_equal.
+    apply Map.ext; intro j.
+    destruct (ident_eq i j).
+    - subst.
+      rewrite Map.gss; auto.
+    - rewrite Map.gso by auto.
+      auto.
+  + unfold obox; simpl.
+    apply andp_left1.
+    apply derives_refl'.
+    f_equal.
+    unfold_lift.
+    destruct rho.
+    f_equal.
+    apply Map.ext; intro j.
+    destruct (ident_eq i j).
+    - subst.
+      rewrite Map.grs; auto.
+    - rewrite Map.gro by auto.
+      auto.
+Qed.
+
+Lemma subst_odia: forall i P,
+  EX v: val, subst i (`v) P = odia i P && (fun rho => !! (Map.get (te_of rho) i <> None)).
+Proof.
+  intros.
+  unfold odia.
+  apply pred_ext.
+  + apply andp_right.
+    - apply orp_right2, derives_refl.
+    - apply exp_left; intros v rho.
+      unfold_lift; unfold subst.
+      unfold env_set.
+      Abort.
+Definition oboxopt ret P :=
+  match ret with
+  | Some id => obox id P
+  | _ => P
+  end.
+
+Lemma substopt_oboxopt: forall id v (P: environ -> mpred), substopt id (`v) (oboxopt id P) = oboxopt id P.
+Proof.
+  intros.
+  destruct id; [| auto].
+  apply subst_obox.
+Qed.
+
+Lemma oboxopt_T: forall i (P: environ -> mpred),
+  oboxopt i P |-- P.
+Proof.
+  intros.
+  destruct i; [| apply derives_refl].
+  apply obox_T.
+Qed.
+
 (* Aux *)
 
 Lemma local_andp_bupd: forall P Q,
@@ -136,6 +263,27 @@ intros; eapply semax_pre_post; try eassumption.
 apply andp_left2; auto.
 Qed.
 
+Lemma semax_post': forall R' Espec {cs: compspecs} Delta R P c,
+           local (tc_environ Delta) && R' |-- R ->
+      @semax cs Espec Delta P c (normal_ret_assert R') ->
+      @semax cs Espec Delta P c (normal_ret_assert R).
+Proof. intros. eapply semax_post; eauto.
+ simpl RA_normal; auto.
+ simpl RA_break; normalize.
+ simpl RA_continue; normalize.
+ intro vl; simpl RA_return; normalize.
+Qed.
+
+Lemma semax_pre_post': forall P' R' Espec {cs: compspecs} Delta R P c,
+      local (tc_environ Delta) && P |-- P' ->
+      local (tc_environ Delta) && R' |-- R ->
+      @semax cs Espec Delta P' c (normal_ret_assert R') ->
+      @semax cs Espec Delta P c (normal_ret_assert R).
+Proof. intros.
+ eapply semax_pre; eauto.
+ eapply semax_post'; eauto.
+Qed.
+
 (* Copied from canon.v end. *)
 
 End CSHL_ConseqFacts.
@@ -146,11 +294,11 @@ Declare Module CSHL_Def: CLIGHT_SEPARATION_HOARE_LOGIC_DEF.
 
 Import CSHL_Def.
 
-Axiom extract_exists:
+Axiom semax_extract_exists:
   forall {CS: compspecs} {Espec: OracleKind},
-  forall (A : Type)  (P : A -> environ->mpred) c (Delta: tycontext) (R: A -> ret_assert),
-  (forall x, @semax CS Espec Delta (P x) c (R x)) ->
-   @semax CS Espec Delta (EX x:A, P x) c (existential_ret_assert R).
+  forall (A : Type)  (P : A -> environ->mpred) c (Delta: tycontext) (R: ret_assert),
+  (forall x, @semax CS Espec Delta (P x) c R) ->
+   @semax CS Espec Delta (EX x:A, P x) c R.
 
 Axiom semax_extract_later_prop:
   forall {CS: compspecs} {Espec: OracleKind},
@@ -245,28 +393,13 @@ Theorem semax_store_backward: forall {CS: compspecs} {Espec: OracleKind} (Delta:
           (normal_ret_assert P).
 Proof.
   intros.
-  eapply semax_pre_post_bupd; [.. | eapply (extract_exists _ _ _ _ (fun _ => normal_ret_assert P))].
-  + apply andp_left2, bupd_intro.
+  eapply semax_post'; [.. | eapply (semax_extract_exists _ _ _ _ (normal_ret_assert P))].
   + apply andp_left2.
     change (RA_normal (existential_ret_assert (fun _ : share => normal_ret_assert P))) with (EX _: share, P).
-    apply exp_left; intros.
-    apply bupd_intro.
-  + apply andp_left2.
-    change (RA_break (existential_ret_assert (fun _ : share => normal_ret_assert P))) with (EX _: share, FF: environ -> mpred).
-    apply exp_left; intros.
-    apply FF_left.
-  + apply andp_left2.
-    change (RA_continue (existential_ret_assert (fun _ : share => normal_ret_assert P))) with (EX _: share, FF: environ -> mpred).
-    apply exp_left; intros.
-    apply FF_left.
-  + intro.
-    apply andp_left2.
-    change (RA_return (existential_ret_assert (fun _ : share => normal_ret_assert P)) vl) with (EX _: share, FF: environ -> mpred).
-    apply exp_left; intros.
-    apply FF_left.
+    apply derives_refl.
   + intros sh.
     apply semax_extract_prop; intro SH.
-    eapply semax_pre_post_bupd; [apply andp_left2, bupd_intro | .. | eapply semax_store_forward; auto].
+    eapply semax_post_bupd; [.. | eapply semax_store_forward; auto].
     - apply andp_left2.
       apply modus_ponens_wand.
     - apply andp_left2, FF_left.
@@ -315,3 +448,154 @@ Proof.
 Qed.
 
 End CSHL_StoreB2F.
+
+Module Type CLIGHT_SEPARATION_HOARE_LOGIC_CALL_FORWARD.
+
+Declare Module CSHL_Def: CLIGHT_SEPARATION_HOARE_LOGIC_DEF.
+
+Import CSHL_Def.
+
+Axiom semax_call_forward: forall {CS: compspecs} {Espec: OracleKind} (Delta: tycontext),
+    forall A P Q NEP NEQ ts x (F: environ -> mpred) ret argsig retsig cc a bl,
+           Cop.classify_fun (typeof a) =
+           Cop.fun_case_f (type_of_params argsig) retsig cc ->
+           (retsig = Tvoid -> ret = None) ->
+          tc_fn_return Delta ret retsig ->
+  @semax CS Espec Delta
+          ((|>((tc_expr Delta a) && (tc_exprlist Delta (snd (split argsig)) bl)))  &&
+         (`(func_ptr (mk_funspec  (argsig,retsig) cc A P Q NEP NEQ)) (eval_expr a) &&
+          |>(F * `(P ts x: environ -> mpred) (make_args' (argsig,retsig) (eval_exprlist (snd (split argsig)) bl)))))
+         (Scall ret a bl)
+         (normal_ret_assert
+            (EX old:val, substopt ret (`old) F * maybe_retval (Q ts x) retsig ret)).
+
+End CLIGHT_SEPARATION_HOARE_LOGIC_CALL_FORWARD.
+
+Module Type CLIGHT_SEPARATION_HOARE_LOGIC_CALL_BACKWARD.
+
+Declare Module CSHL_Def: CLIGHT_SEPARATION_HOARE_LOGIC_DEF.
+
+Import CSHL_Def.
+
+Axiom semax_call_backward: forall {CS: compspecs} {Espec: OracleKind} (Delta: tycontext),
+    forall ret a bl R,
+  @semax CS Espec Delta
+         (EX argsig: _, EX retsig: _, EX cc: _,
+          EX A: _, EX P: _, EX Q: _, EX NEP: _, EX NEQ: _, EX ts: _, EX x: _,
+         !! (Cop.classify_fun (typeof a) =
+             Cop.fun_case_f (type_of_params argsig) retsig cc /\
+             (retsig = Tvoid -> ret = None) /\
+             tc_fn_return Delta ret retsig) &&
+          (|>((tc_expr Delta a) && (tc_exprlist Delta (snd (split argsig)) bl)))  &&
+         `(func_ptr (mk_funspec  (argsig,retsig) cc A P Q NEP NEQ)) (eval_expr a) &&
+          |>((`(P ts x: environ -> mpred) (make_args' (argsig,retsig) (eval_exprlist (snd (split argsig)) bl))) * oboxopt ret (maybe_retval (Q ts x) retsig ret -* R)))
+         (Scall ret a bl)
+         (normal_ret_assert R).
+
+End CLIGHT_SEPARATION_HOARE_LOGIC_CALL_BACKWARD.
+
+Module CSHL_CallF2B
+       (CSHL_Def: CLIGHT_SEPARATION_HOARE_LOGIC_DEF)
+       (CSHL_Conseq: CLIGHT_SEPARATION_HOARE_LOGIC_CONSEQUENCE with Module CSHL_Def := CSHL_Def)
+       (CSHL_Extr: CLIGHT_SEPARATION_HOARE_LOGIC_EXTRACTION with Module CSHL_Def := CSHL_Def)
+       (CSHL_CallF: CLIGHT_SEPARATION_HOARE_LOGIC_CALL_FORWARD with Module CSHL_Def := CSHL_Def):
+       CLIGHT_SEPARATION_HOARE_LOGIC_CALL_BACKWARD.
+
+Module CSHL_Def := CSHL_Def.
+Module CSHL_ConseqFacts := CSHL_ConseqFacts (CSHL_Def) (CSHL_Conseq).
+Module CSHL_ExtrFacts := CSHL_ExtrFacts (CSHL_Def) (CSHL_Conseq) (CSHL_Extr).
+Import CSHL_Def.
+Import CSHL_Conseq.
+Import CSHL_ConseqFacts.
+Import CSHL_Extr.
+Import CSHL_ExtrFacts.
+Import CSHL_CallF.
+  
+Theorem semax_call_backward: forall {CS: compspecs} {Espec: OracleKind} (Delta: tycontext),
+    forall ret a bl R,
+  @semax CS Espec Delta
+         (EX argsig: _, EX retsig: _, EX cc: _,
+          EX A: _, EX P: _, EX Q: _, EX NEP: _, EX NEQ: _, EX ts: _, EX x: _,
+         !! (Cop.classify_fun (typeof a) =
+             Cop.fun_case_f (type_of_params argsig) retsig cc /\
+             (retsig = Tvoid -> ret = None) /\
+             tc_fn_return Delta ret retsig) &&
+          (|>((tc_expr Delta a) && (tc_exprlist Delta (snd (split argsig)) bl)))  &&
+         `(func_ptr (mk_funspec  (argsig,retsig) cc A P Q NEP NEQ)) (eval_expr a) &&
+          |>((`(P ts x: environ -> mpred) (make_args' (argsig,retsig) (eval_exprlist (snd (split argsig)) bl))) * oboxopt ret (maybe_retval (Q ts x) retsig ret -* R)))
+         (Scall ret a bl)
+         (normal_ret_assert R).
+Proof.
+  intros.
+  apply semax_extract_exists; intro argsig.
+  apply semax_extract_exists; intro retsig.
+  apply semax_extract_exists; intro cc.
+  apply semax_extract_exists; intro A.
+  apply semax_extract_exists; intro P.
+  apply semax_extract_exists; intro Q.
+  apply semax_extract_exists; intro NEP.
+  apply semax_extract_exists; intro NEQ.
+  apply semax_extract_exists; intro ts.
+  apply semax_extract_exists; intro x.
+  rewrite !andp_assoc.
+  apply semax_extract_prop; intros [? [? ?]].
+  eapply semax_pre_post'; [.. | apply semax_call_forward; auto].
+  + apply andp_left2.
+    apply andp_derives; [apply derives_refl |].
+    apply andp_derives; [apply derives_refl |].
+    apply later_derives.
+    rewrite sepcon_comm.
+    apply derives_refl.
+  + unfold RA_normal, normal_ret_assert.
+    apply andp_left2.
+    apply exp_left; intro old.
+    rewrite wand_sepcon_adjoint.
+    rewrite substopt_oboxopt.
+    apply oboxopt_T.
+  + auto.
+  + auto.
+  + auto.
+Qed.
+
+End CSHL_CallF2B.
+
+Module CSHL_CallB2F
+       (CSHL_Def: CLIGHT_SEPARATION_HOARE_LOGIC_DEF)
+       (CSHL_Conseq: CLIGHT_SEPARATION_HOARE_LOGIC_CONSEQUENCE with Module CSHL_Def := CSHL_Def)
+       (CSHL_CallB: CLIGHT_SEPARATION_HOARE_LOGIC_CALL_BACKWARD with Module CSHL_Def := CSHL_Def):
+       CLIGHT_SEPARATION_HOARE_LOGIC_CALL_FORWARD.
+
+Module CSHL_Def := CSHL_Def.
+Module CSHL_ConseqFacts := CSHL_ConseqFacts (CSHL_Def) (CSHL_Conseq).
+Import CSHL_Def.
+Import CSHL_Conseq.
+Import CSHL_ConseqFacts.
+Import CSHL_CallB.
+
+Theorem semax_call_forward: forall {CS: compspecs} {Espec: OracleKind} (Delta: tycontext),
+    forall A P Q NEP NEQ ts x (F: environ -> mpred) ret argsig retsig cc a bl,
+           Cop.classify_fun (typeof a) =
+           Cop.fun_case_f (type_of_params argsig) retsig cc ->
+           (retsig = Tvoid -> ret = None) ->
+          tc_fn_return Delta ret retsig ->
+  @semax CS Espec Delta
+          ((|>((tc_expr Delta a) && (tc_exprlist Delta (snd (split argsig)) bl)))  &&
+         (`(func_ptr (mk_funspec  (argsig,retsig) cc A P Q NEP NEQ)) (eval_expr a) &&
+          |>(F * `(P ts x: environ -> mpred) (make_args' (argsig,retsig) (eval_exprlist (snd (split argsig)) bl)))))
+         (Scall ret a bl)
+         (normal_ret_assert
+            (EX old:val, substopt ret (`old) F * maybe_retval (Q ts x) retsig ret)).
+Proof.
+  intros.
+  eapply semax_pre; [| apply semax_call_backward].
+  apply (exp_right argsig), (exp_right retsig), (exp_right cc), (exp_right A), (exp_right P), (exp_right Q), (exp_right NEP), (exp_right NEQ), (exp_right ts), (exp_right x).
+  apply andp_left2.
+  rewrite !andp_assoc.
+  apply andp_right; [apply prop_right; auto |].
+  apply andp_derives; auto.
+  apply andp_derives; auto.
+  apply later_derives.
+  rewrite sepcon_comm.
+  apply sepcon_derives; auto.
+  Print tc_environ.
+  Print typecheck_environ.
